CollapsingTowers/TwoLevelPCP/Typing.lean
@@ -12,75 +12,68 @@ def well_binding_time : Stage → Ty → Prop
   | .dyn, (.arrow τ𝕒 τ𝕓 φ) => φ = ∅ ∧ well_binding_time .dyn τ𝕒 ∧ well_binding_time .dyn τ𝕓
   | .dyn, _ => false
 
-@[simp]
-def well_reification : Ty → Effects → Prop
-  | _, .pure => true
-  | .rep _, .reflect => true
-  | _, _ => false
+mutual
+  inductive typing : TEnv → Stage → Expr → Ty → Effects → Prop where
+    | fvar : ∀ Γ 𝕊 x τ,
+      binds x τ 𝕊 Γ →
+      typing Γ 𝕊 (.fvar x) τ ∅
+    | lam₁ : ∀ Γ 𝕊 e τ𝕒 τ𝕓 φ,
+      typing ((τ𝕒, 𝕊) :: Γ) 𝕊 (open₀ Γ.length e) τ𝕓 φ →
+      well_binding_time 𝕊 τ𝕒 →
+      closed_at e Γ.length →
+      typing Γ 𝕊 (.lam₁ e) (.arrow τ𝕒 τ𝕓 φ) ∅
+    | lift_lam : ∀ Γ e τ𝕒 τ𝕓 φ₀ φ₁,
+      typing Γ .stat e (.arrow (.fragment τ𝕒) (.fragment τ𝕓) φ₀) φ₁ →
+      typing Γ .stat (.lift e) (.fragment (.arrow τ𝕒 τ𝕓 ∅)) .reflect
+    | app₁ : ∀ Γ 𝕊 f arg τ𝕒 τ𝕓 φ₀ φ₁ φ₂,
+      typing Γ 𝕊 f (.arrow τ𝕒 τ𝕓 φ₀) φ₁ →
+      typing Γ 𝕊 arg τ𝕒 φ₂ →
+      typing Γ 𝕊 (.app₁ f arg) τ𝕓 (φ₀ ∪ φ₁ ∪ φ₂)
+    | app₂ : ∀ Γ f arg τ𝕒 τ𝕓 φ₀ φ₁,
+      typing Γ .stat f (.fragment (.arrow τ𝕒 τ𝕓 ∅)) φ₀ →
+      typing Γ .stat arg (.fragment τ𝕒) φ₁ →
+      typing Γ .stat (.app₂ f arg) (.fragment τ𝕓) .reflect
+    | plus₁ : ∀ Γ 𝕊 l r φ₀ φ₁,
+      typing Γ 𝕊 l .nat φ₀ →
+      typing Γ 𝕊 r .nat φ₁ →
+      typing Γ 𝕊 (.plus₁ l r) .nat (φ₀ ∪ φ₁)
+    | plus₂ : ∀ Γ l r φ₀ φ₁,
+      typing Γ .stat l (.fragment .nat) φ₀ →
+      typing Γ .stat r (.fragment .nat) φ₁ →
+      typing Γ .stat (.plus₂ l r) (.fragment .nat) .reflect
+    | lit₁ : ∀ Γ 𝕊 n,
+      typing Γ 𝕊 (.lit₁ n) .nat ∅
+    | lift_lit : ∀ Γ n φ,
+      typing Γ .stat n .nat φ →
+      typing Γ .stat (.lift n) (.fragment .nat) φ
+    | code₁ : ∀ Γ x τ,
+      binds x τ .dyn Γ →
+      typing Γ .stat (.code (.fvar x)) (.fragment τ) ∅
+    | code₂ : ∀ Γ e τ,
+      typing Γ .dyn e τ ∅ →
+      typing Γ .stat (.code e) (.rep τ) ∅
+    | reflect : ∀ Γ e τ,
+      typing Γ .dyn e τ ∅ →
+      typing Γ .stat (.reflect e) (.fragment τ) .reflect
+    | lam𝕔 : ∀ Γ e τ𝕒 τ𝕓,
+      typing_reification ((τ𝕒, .dyn) :: Γ) (open₀ Γ.length e) (.rep τ𝕓) →
+      well_binding_time .dyn τ𝕒 →
+      closed_at e Γ.length →
+      typing Γ .stat (.lam𝕔 e) (.fragment (.arrow τ𝕒 τ𝕓 ∅)) .reflect
+    | lets : ∀ Γ 𝕊 b e τ𝕒 τ𝕓 φ₀ φ₁,
+      typing Γ 𝕊 b τ𝕒 φ₀ →
+      typing ((τ𝕒, 𝕊) :: Γ) 𝕊 (open₀ Γ.length e) τ𝕓 φ₁ →
+      well_binding_time 𝕊 τ𝕒 →
+      closed_at e Γ.length →
+      typing Γ 𝕊 (.lets b e) τ𝕓 (φ₀ ∪ φ₁)
+    | let𝕔 : ∀ Γ b e τ𝕒 τ𝕓,
+      typing Γ .dyn b τ𝕒 ∅ →
+      typing_reification ((τ𝕒, .dyn) :: Γ) (open₀ Γ.length e) (.rep τ𝕓) →
+      well_binding_time .dyn τ𝕒 →
+      closed_at e Γ.length →
+      typing Γ .stat (.let𝕔 b e) (.rep τ𝕓) ∅
 
-inductive typing : TEnv → Stage → Expr → Ty → Effects → Prop where
-  | fvar : ∀ Γ 𝕊 x τ,
-    binds x τ 𝕊 Γ →
-    typing Γ 𝕊 (.fvar x) τ ∅
-  | lam₁ : ∀ Γ 𝕊 e τ𝕒 τ𝕓 φ,
-    typing ((τ𝕒, 𝕊) :: Γ) 𝕊 (open₀ Γ.length e) τ𝕓 φ →
-    well_binding_time 𝕊 τ𝕒 →
-    closed_at e Γ.length →
-    typing Γ 𝕊 (.lam₁ e) (.arrow τ𝕒 τ𝕓 φ) ∅
-  | lift_lam : ∀ Γ e τ𝕒 τ𝕓 φ₀ φ₁,
-    typing Γ .stat e (.arrow (.fragment τ𝕒) (.fragment τ𝕓) φ₀) φ₁ →
-    typing Γ .stat (.lift e) (.fragment (.arrow τ𝕒 τ𝕓 ∅)) .reflect
-  | app₁ : ∀ Γ 𝕊 f arg τ𝕒 τ𝕓 φ₀ φ₁ φ₂,
-    typing Γ 𝕊 f (.arrow τ𝕒 τ𝕓 φ₀) φ₁ →
-    typing Γ 𝕊 arg τ𝕒 φ₂ →
-    typing Γ 𝕊 (.app₁ f arg) τ𝕓 (φ₀ ∪ φ₁ ∪ φ₂)
-  | app₂ : ∀ Γ f arg τ𝕒 τ𝕓 φ₀ φ₁,
-    typing Γ .stat f (.fragment (.arrow τ𝕒 τ𝕓 ∅)) φ₀ →
-    typing Γ .stat arg (.fragment τ𝕒) φ₁ →
-    typing Γ .stat (.app₂ f arg) (.fragment τ𝕓) .reflect
-  | plus₁ : ∀ Γ 𝕊 l r φ₀ φ₁,
-    typing Γ 𝕊 l .nat φ₀ →
-    typing Γ 𝕊 r .nat φ₁ →
-    typing Γ 𝕊 (.plus₁ l r) .nat (φ₀ ∪ φ₁)
-  | plus₂ : ∀ Γ l r φ₀ φ₁,
-    typing Γ .stat l (.fragment .nat) φ₀ →
-    typing Γ .stat r (.fragment .nat) φ₁ →
-    typing Γ .stat (.plus₂ l r) (.fragment .nat) .reflect
-  | lit₁ : ∀ Γ 𝕊 n,
-    typing Γ 𝕊 (.lit₁ n) .nat ∅
-  | lift_lit : ∀ Γ n φ,
-    typing Γ .stat n .nat φ →
-    typing Γ .stat (.lift n) (.fragment .nat) φ
-  | code₁ : ∀ Γ x τ,
-    binds x τ .dyn Γ →
-    typing Γ .stat (.code (.fvar x)) (.fragment τ) ∅
-  | code₂ : ∀ Γ e τ,
-    typing Γ .dyn e τ ∅ →
-    typing Γ .stat (.code e) (.rep τ) ∅
-  | lift_code : ∀ Γ e τ φ,
-    typing Γ .stat e (.fragment τ) φ →
-    typing Γ .stat e (.rep τ) φ
-  | reflect : ∀ Γ e τ,
-    typing Γ .dyn e τ ∅ →
-    typing Γ .stat (.reflect e) (.fragment τ) .reflect
-  | lam𝕔 : ∀ Γ e τ𝕒 τ𝕓 φ,
-    typing ((τ𝕒, .dyn) :: Γ) .stat (open₀ Γ.length e) (.rep τ𝕓) φ →
-    well_binding_time .dyn τ𝕒 →
-    closed_at e Γ.length →
-    typing Γ .stat (.lam𝕔 e) (.fragment (.arrow τ𝕒 τ𝕓 ∅)) .reflect
-  | lets : ∀ Γ 𝕊 b e τ𝕒 τ𝕓 φ₀ φ₁,
-    typing Γ 𝕊 b τ𝕒 φ₀ →
-    typing ((τ𝕒, 𝕊) :: Γ) 𝕊 (open₀ Γ.length e) τ𝕓 φ₁ →
-    well_binding_time 𝕊 τ𝕒 →
-    closed_at e Γ.length →
-    typing Γ 𝕊 (.lets b e) τ𝕓 (φ₀ ∪ φ₁)
-  | let𝕔 : ∀ Γ b e τ𝕒 τ𝕓 φ,
-    typing Γ .dyn b τ𝕒 ∅ →
-    typing ((τ𝕒, .dyn) :: Γ) .stat (open₀ Γ.length e) (.rep τ𝕓) φ →
-    well_binding_time .dyn τ𝕒 →
-    closed_at e Γ.length →
-    typing Γ .stat (.let𝕔 b e) (.rep τ𝕓) ∅
-
-@[simp]
-def typing_reification (Γ : TEnv) (e : Expr) (τ : Ty) (φ : Effects) : Prop :=
-  typing Γ .stat e τ φ ∧ well_reification τ φ
+  inductive typing_reification : TEnv → Expr → Ty → Prop
+    | pure : ∀ Γ e τ, typing Γ .stat e τ ∅ -> typing_reification Γ e τ
+    | reflect : ∀ Γ e τ, typing Γ .stat e (.fragment τ) .reflect -> typing_reification Γ e (.rep τ)
+end
