CollapsingTowers/TwoLevelPCP/Example.lean
@@ -62,98 +62,178 @@ def expr𝕩 : Expr :=
 def τ : Ty :=
   .rep (.arrow .nat .nat ∅)
 
-example : typing_reification [] expr₀ τ .reflect := by
+example : typing_reification [] expr₀ τ := by
   rw [expr₀, x₀, τ]
-  repeat
-    ( try rw [← union_empty ∅]
-      constructor)
-
-example : typing_reification [] expr₁ τ .reflect := by
-  rw [expr₁, x₀, τ]
-  repeat
-    ( try rw [← union_empty ∅]
-      constructor)
-
-example : typing_reification [] expr₂ τ .reflect := by
-  rw [expr₂, x₀, τ]
-  repeat
-    ( try rw [← union_empty ∅]
-      constructor)
-
-example : typing_reification [] expr₃ τ .reflect := by
-  rw [expr₃, x₀, x₁, τ]
-  constructor
-  apply typing.lift_code
-  apply typing.lam𝕔
-  apply typing.let𝕔
-  repeat
-    ( try rw [← union_empty ∅]
-      constructor)
-
-example : typing_reification [] expr₄ τ .reflect := by
-  rw [expr₄, x₀, x₁, τ]
-  constructor
-  apply typing.lift_code
-  apply typing.lam𝕔
-  apply typing.let𝕔
-  repeat
-    ( try rw [← union_empty ∅]
-      constructor)
-
-example : typing_reification [] expr₅ τ .reflect := by
-  rw [expr₅, x₀, x₁, x₂, τ]
-  constructor
-  apply typing.lift_code
-  apply typing.lam𝕔
-  apply typing.let𝕔;
-  .
-    repeat
-      ( try rw [← union_empty ∅]
-        constructor)
-  apply typing.let𝕔;
-  .
-    repeat
-      ( try rw [← union_empty ∅]
-        constructor)
+  apply typing_reification.reflect
+  apply typing.lift_lam
+  apply typing.lam₁
+  apply typing.plus₂
+  apply typing.fvar; . repeat constructor
+  apply typing.plus₂
+  apply typing.fvar; . repeat constructor
+  apply typing.fvar; . repeat constructor
   repeat constructor
 
-example : typing_reification [] expr₆ τ .reflect := by
-  rw [expr₆, x₀, x₁, x₂, τ]
-  constructor
-  apply typing.lift_code
+example : typing_reification [] expr₁ τ := by
+  rw [expr₁, x₀, τ]
+  apply typing_reification.reflect
   apply typing.lam𝕔
-  apply typing.let𝕔
-  repeat
-    ( try rw [← union_empty ∅]
-      constructor)
+  apply typing_reification.reflect
+  apply typing.plus₂
+  apply typing.code₁; . repeat constructor
+  apply typing.plus₂
+  apply typing.code₁; . repeat constructor
+  apply typing.code₁; . repeat constructor
+  repeat constructor
 
-example : typing_reification [] expr₇ τ .reflect := by
-  rw [expr₇, x₀, x₁, x₂, τ]
-  repeat
-    ( try rw [← union_empty ∅]
-      constructor)
+example : typing_reification [] expr₂ τ := by
+  rw [expr₂, x₀, τ]
+  apply typing_reification.reflect
+  apply typing.lam𝕔
+  apply typing_reification.reflect
+  apply typing.plus₂
+  apply typing.code₁; . repeat constructor
+  apply typing.reflect; rw [← union_empty ∅]
+  apply typing.plus₁
+  apply typing.fvar; . repeat constructor
+  apply typing.fvar; . repeat constructor
+  repeat constructor
 
-example : typing_reification [] expr₈ τ .reflect := by
-  rw [expr₈, x₀, x₁, x₂, τ]
-  repeat
-    ( try rw [← union_empty ∅]
-      constructor)
+example : typing_reification [] expr₃ τ := by
+  rw [expr₃, x₀, x₁, τ]
+  apply typing_reification.reflect
+  apply typing.lam𝕔
+  apply typing_reification.pure
+  apply typing.let𝕔; rw [← union_empty ∅]
+  apply typing.plus₁
+  apply typing.fvar; . repeat constructor
+  apply typing.fvar; . repeat constructor
+  apply typing_reification.reflect
+  apply typing.plus₂
+  apply typing.code₁; . repeat constructor
+  apply typing.code₁; . repeat constructor
+  repeat constructor
 
-example : typing_reification [] expr₉ τ ∅ := by
-  rw [expr₉, x₀, x₁, x₂, τ]
-  constructor
-  apply typing.let𝕔
-  repeat
-    ( try rw [← union_empty ∅]
-      constructor)
+example : typing_reification [] expr₄ τ := by
+  rw [expr₄, x₀, x₁, τ]
+  apply typing_reification.reflect
+  apply typing.lam𝕔
+  apply typing_reification.pure
+  apply typing.let𝕔; rw [← union_empty ∅]
+  apply typing.plus₁
+  apply typing.fvar; . repeat constructor
+  apply typing.fvar; . repeat constructor
+  apply typing_reification.reflect
+  apply typing.reflect; rw [← union_empty ∅]
+  apply typing.plus₁
+  apply typing.fvar; . repeat constructor
+  apply typing.fvar; . repeat constructor
+  repeat constructor
 
-example : typing_reification [] expr𝕩 τ ∅ := by
-  rw [expr𝕩, x₀, x₁, x₂, τ]
-  constructor
+example : typing_reification [] expr₅ τ := by
+  rw [expr₅, x₀, x₁, x₂, τ]
+  apply typing_reification.reflect
+  apply typing.lam𝕔
+  apply typing_reification.pure
+  apply typing.let𝕔; rw [← union_empty ∅]
+  apply typing.plus₁
+  apply typing.fvar; . repeat constructor
+  apply typing.fvar; . repeat constructor
+  apply typing_reification.pure
+  apply typing.let𝕔; rw [← union_empty ∅]
+  apply typing.plus₁
+  apply typing.fvar; . repeat constructor
+  apply typing.fvar; . repeat constructor
+  apply typing_reification.pure
   apply typing.code₂
-  repeat
-    ( try rw [← union_empty ∅]
-      constructor)
+  apply typing.fvar; . repeat constructor
+  repeat constructor
+
+example : typing_reification [] expr₆ τ := by
+  rw [expr₆, x₀, x₁, x₂, τ]
+  apply typing_reification.reflect
+  apply typing.lam𝕔
+  apply typing_reification.pure
+  apply typing.let𝕔; rw [← union_empty ∅]
+  apply typing.plus₁
+  apply typing.fvar; . repeat constructor
+  apply typing.fvar; . repeat constructor
+  apply typing_reification.pure
+  apply typing.code₂; rw [← union_empty ∅]
+  apply typing.lets; rw [← union_empty ∅]
+  apply typing.plus₁
+  apply typing.fvar; . repeat constructor
+  apply typing.fvar; . repeat constructor
+  apply typing.fvar; . repeat constructor
+  repeat constructor
+
+example : typing_reification [] expr₇ τ := by
+  rw [expr₇, x₀, x₁, x₂, τ]
+  apply typing_reification.reflect
+  apply typing.lam𝕔
+  apply typing_reification.pure
+  apply typing.code₂; rw [← union_empty ∅]
+  apply typing.lets; rw [← union_empty ∅]
+  apply typing.plus₁
+  apply typing.fvar; . repeat constructor
+  apply typing.fvar; . repeat constructor
+  rw [← union_empty ∅]
+  apply typing.lets; rw [← union_empty ∅]
+  apply typing.plus₁
+  apply typing.fvar; . repeat constructor
+  apply typing.fvar; . repeat constructor
+  apply typing.fvar; . repeat constructor
+  repeat constructor
+
+example : typing_reification [] expr₈ τ := by
+  rw [expr₈, x₀, x₁, x₂, τ]
+  apply typing_reification.reflect
+  apply typing.reflect
+  apply typing.lam₁; rw [← union_empty ∅]
+  apply typing.lets; rw [← union_empty ∅]
+  apply typing.plus₁
+  apply typing.fvar; . repeat constructor
+  apply typing.fvar; . repeat constructor
+  rw [← union_empty ∅]
+  apply typing.lets; rw [← union_empty ∅]
+  apply typing.plus₁
+  apply typing.fvar; . repeat constructor
+  apply typing.fvar; . repeat constructor
+  apply typing.fvar; . repeat constructor
+  repeat constructor
+
+example : typing_reification [] expr₉ τ := by
+  rw [expr₉, x₀, x₁, x₂, τ]
+  apply typing_reification.pure
+  apply typing.let𝕔
+  apply typing.lam₁
+  apply typing.lets
+  apply typing.plus₁
+  apply typing.fvar; . repeat constructor
+  apply typing.fvar; . repeat constructor
+  apply typing.lets
+  apply typing.plus₁
+  apply typing.fvar; . repeat constructor
+  apply typing.fvar; . repeat constructor
+  apply typing.fvar; . repeat constructor
+  repeat constructor
+
+example : typing_reification [] expr𝕩 τ := by
+  rw [expr𝕩, x₀, x₁, x₂, τ]
+  apply typing_reification.pure
+  apply typing.code₂; rw [← union_empty ∅]
+  apply typing.lets; rw [← union_empty ∅]
+  apply typing.lam₁
+  apply typing.lets
+  apply typing.plus₁
+  apply typing.fvar; . repeat constructor
+  apply typing.fvar; . repeat constructor
+  apply typing.lets
+  apply typing.plus₁
+  apply typing.fvar; . repeat constructor
+  apply typing.fvar; . repeat constructor
+  apply typing.fvar; . repeat constructor
+  repeat constructor
 
 end Example1
 
@@ -162,20 +242,26 @@ namespace PhaseConsistency
 -- stuck example
 -- letc x (* phase 2 *) = eff in
 -- x (* phase 1 *)
-example : ∀ b τ φ, ¬typing_reification [] (.let𝕔 b (.bvar 0)) τ φ :=
+example : ∀ b τ, ¬typing_reification [] (.let𝕔 b (.bvar 0)) τ :=
   by
-  intros _ _ _ Hτ
-  cases Hτ
-  contradiction
+  intros _ _ Hτ
+  cases Hτ <;> contradiction
 
 -- cross stage persistence
 -- let x (* phase 1 *) = ref 0 in
 -- code x (* phase 2 *)
-example : ∀ b τ φ, ¬typing_reification [] (.lets b (.code (.bvar 0))) τ φ :=
+example : ∀ b τ, ¬typing_reification [] (.lets b (.code (.bvar 0))) τ :=
   by
-  intros _ _ _ Hτ
+  intros _ _ Hτ
   cases Hτ
-  contradiction
+  case pure Hτ =>
+    generalize eqφ : (∅ : Effects) = φ
+    rw [eqφ] at Hτ
+    cases Hτ; contradiction
+  case reflect Hτ =>
+    generalize eqφ : (.reflect : Effects) = φ
+    rw [eqφ] at Hτ
+    cases Hτ; contradiction
 
 end PhaseConsistency
 
@@ -186,14 +272,20 @@ namespace Reification
 --    letc x0 = eff in
 --    code x0
 -- in e
-example : ∀ b e τ φ, ¬typing_reification [] (.lets (.let𝕔 b (.code (.bvar 0))) e) τ φ :=
+example : ∀ b e τ, ¬typing_reification [] (.lets (.let𝕔 b (.code (.bvar 0))) e) τ :=
   by
-  intros _ _ _ _ Hτ
-  cases (Hτ.left)
-  case lets Hlet𝕔 _ _ => cases Hlet𝕔 <;> contradiction
-  case lift_code Hτ =>
+  intros _ _ _ Hτ
+  cases Hτ
+  case pure Hτ =>
+    generalize eqφ : (∅ : Effects) = φ
+    rw [eqφ] at Hτ
     cases Hτ
-    case lets Hlet𝕔 _ _ => cases Hlet𝕔 <;> contradiction
+    case lets Hcode _ _ => cases Hcode; contradiction
+  case reflect Hτ =>
+    generalize eqφ : (.reflect : Effects) = φ
+    rw [eqφ] at Hτ
+    cases Hτ
+    case lets Hcode _ _ => cases Hcode; contradiction
 
 -- reify result under B context
 -- let x = code {
@@ -201,25 +293,39 @@ example : ∀ b e τ φ, ¬typing_reification [] (.lets (.let𝕔 b (.code (.bva
 --    x0
 -- }
 -- in e
-example : ∀ b e τ φ, ¬typing_reification [] (.lets (.code (.lets b (.bvar 0))) e) τ φ :=
+example : ∀ b e τ, ¬typing_reification [] (.lets (.code (.lets b (.bvar 0))) e) τ :=
   by
-  intros _ _ _ _ Hτ
-  cases (Hτ.left)
-  case lets Hcode _ _ => cases Hcode <;> contradiction
-  case lift_code Hτ =>
+  intros _ _ _ Hτ
+  cases Hτ
+  case pure Hτ =>
+    generalize eqφ : (∅ : Effects) = φ
+    rw [eqφ] at Hτ
     cases Hτ
-    case lets Hlet𝕔 _ _ => cases Hlet𝕔 <;> contradiction
+    case lets Hcode _ _ => cases Hcode; contradiction
+  case reflect Hτ =>
+    generalize eqφ : (.reflect : Effects) = φ
+    rw [eqφ] at Hτ
+    cases Hτ
+    case lets Hcode _ _ => cases Hcode; contradiction
 
 -- E context must has resulting type rep τ -> rep τ
 -- let x = reflect e
 -- in 1
-example : ∀ e τ φ, ¬typing_reification [] (.lets (.reflect e) (.lit₁ 1)) τ φ :=
+example : ∀ e τ, ¬typing_reification [] (.lets (.reflect e) (.lit₁ 1)) τ :=
   by
-  intros _ _ _ Hτ
-  cases (Hτ.left) <;> try contradiction
-  case lets Hreflect _ Hlit₁ =>
-    cases Hlit₁ <;> try contradiction
-    cases Hreflect <;> try contradiction
-    nomatch (Hτ.right)
+  intros _ _ Hτ
+  cases Hτ
+  case pure Hτ =>
+    generalize eqφ : (∅ : Effects) = φ
+    rw [eqφ] at Hτ
+    cases Hτ
+    case lets Hreflect _ _ =>
+      cases Hreflect
+      simp at eqφ
+  case reflect Hτ =>
+    generalize eqφ : (.reflect : Effects) = φ
+    rw [eqφ] at Hτ
+    cases Hτ
+    case lets Hreflect _ _ => cases Hreflect; contradiction
 
 end Reification
